.

theories/Prelude/Prelude.v
@@ -1153,6 +1153,8 @@ Class retracts (X : Type) (P : Prop) : Type :=
   ; retraction : P -> X
   ; retraction_section (x : X)
     : retraction (section x) = x
+  ; section_retraction (H : P)
+    : section (retraction H) = H
   }.
 
 Definition Prop_to_Set (P : Prop) : Set :=
@@ -1163,6 +1165,7 @@ Instance trivial_retraction (P : Prop) : retracts (Prop_to_Set P) P :=
   { section (x : Prop_to_Set P) := x
   ; retraction (H : P) := H
   ; retraction_section := @eq_refl (Prop_to_Set P)
+  ; section_retraction := @eq_refl (Prop_to_Set P)
   }.
 
 End B.
